<?xml version="1.0" encoding="UTF-8"?>
<rdf:RDF xml:base="http://canlink.library.ualberta.ca/ontologies/canlink#" 
  xmlns="http://canlink.library.ualberta.ca/ontologies/canlink#" 
  xmlns:as="http://www.w3.org/ns/activitystreams#" 
  xmlns:bio="http://purl.org/vocab/bio/0.1/" 
  xmlns:cc="http://creativecommons.org/ns#" 
  xmlns:cwrc="http://canlink.library.ualberta.ca/ontologies/canlink#" 
  xmlns:dbpedia="http://dbpedia.org/resource/" 
  xmlns:dcterms="http://purl.org/dc/terms/" 
  xmlns:frbr="http://purl.org/vocab/frbr/core#"
  xmlns:doap="http://usefulinc.com/ns/doap#" 
  xmlns:bibo="http://purl.org/ontology/bibo/"
  xmlns:foaf="http://xmlns.com/foaf/0.1/" 
  xmlns:loc="http://id.loc.gov/vocabulary/relators/" 
  xmlns:locl ="http://id.loc.gov/vocabulary/languages/"
  xmlns:nif="http://persistence.uni-leipzig.org/nlp2rdf/ontologies/nif-core#" 
  xmlns:oa="http://www.w3.org/ns/oa#" 
  xmlns:owl="http://www.w3.org/2002/07/owl#" 
  xmlns:prov="http://www.w3.org/ns/prov#" 
  xmlns:rdf="http://www.w3.org/1999/02/22-rdf-syntax-ns#" 
  xmlns:rdfs="http://www.w3.org/2000/01/rdf-schema#" 
  xmlns:rel="http://purl.org/vocab/relationship/" 
  xmlns:skos="http://www.w3.org/2004/02/skos/core#" 
  xmlns:skosxl="http://www.w3.org/2008/05/skos-xl#" 
  xmlns:time="http://www.w3.org/2006/time#" 
  xmlns:vann="http://purl.org/vocab/vann/" 
  xmlns:voaf="http://purl.org/vocommons/voaf#" 
  xmlns:genre="http://sparql.cwrc.ca/ontologies/genre#"
  xmlns:void="http://rdfs.org/ns/void#" 
  xmlns:vs="http://www.w3.org/2003/06/sw-vocab-status/ns#" 
  xmlns:xsd="http://www.w3.org/2001/XMLSchema#">

  <owl:Ontology rdf:about="">
    <rdf:type rdf:resource="http://purl.org/vocommons/voaf#Vocabulary"/>
    <dcterms:title xml:lang="en">The CanLink Ontology</dcterms:title>
    <rdfs:label xml:lang="en">The CanLink Ontology</rdfs:label>
    <foaf:name xml:lang="en">The CanLink Ontology</foaf:name>
    <dcterms:title xml:lang="fr">L'Ontologie CanLien</dcterms:title>
    <rdfs:label xml:lang="fr">L'Ontologie CanLien</rdfs:label>
    <foaf:name xml:lang="fr">L'Ontologie CanLien</foaf:name>
    <dcterms:description xml:lang="en">The CanLink ontology ties together several vocabularies to represent a Canadian thesis collection.</dcterms:description>
    <skos:definition xml:lang="en">The CanLink ontology ties together several vocabularies to represent a Canadian thesis collection.</skos:definition>
    <rdfs:comment xml:lang="en">The CanLink ontology ties together several vocabularies to represent a Canadian thesis collection.</rdfs:comment>
    <dcterms:description xml:lang="fr">L'ontologie CanLien lie plusieurs vocabulaires pour représenter une collection de thèses canadiennes.</dcterms:description>
    <skos:definition xml:lang="fr">L'ontologie CanLien lie plusieurs vocabulaires pour représenter une collection de thèses canadiennes.</skos:definition>
    <rdfs:comment xml:lang="fr">L'ontologie CanLien lie plusieurs vocabulaires pour représenter une collection de thèses canadiennes.</rdfs:comment>
    <owl:versionInfo>1.0</owl:versionInfo>
    <dcterms:date rdf:datatype="http://www.w3.org/2001/XMLSchema#date">DATE_TODAY</dcterms:date>
    <dcterms:rights rdf:resource="http://creativecommons.org/licenses/by-nc/4.0/"/>
    <vs:term_status xml:lang="en">Stable</vs:term_status>
    <dcterms:creator>
      <foaf:Person rdf:about="#RobWarren">
        <foaf:name>Robert Warren</foaf:name>
        <owl:sameAs rdf:resource="http://rdf.muninn-project.org/ww1/2011/11/11/Person/Warren"/>
        <owl:sameAs rdf:resource="http://sparql.cwrc.ca/ontology/cwrc#RobWarren"/>
      </foaf:Person>
    </dcterms:creator>
    <dcterms:creator>
      <foaf:Person rdf:about="#SharonFarnel">
        <foaf:name>Sharon Farnel</foaf:name>
      </foaf:Person>
    </dcterms:creator>
    <dcterms:creator>
      <foaf:Person rdf:about="#MaharshPatel">
        <foaf:name>Maharsh Patel</foaf:name>
      </foaf:Person>
    </dcterms:creator>
    <dcterms:publisher rdf:resource="#CLDI"/>
    <void:inDataset rdf:resource="#datasetdefinition"/>
    <rdfs:isDefinedBy rdf:resource="http://canlink.library.ualberta.ca/ontologies/canlink"/>
    <!-- Electronic dissertations  -->
    <dcterms:subject rdf:resource="http://id.loc.gov/authorities/subjects/sh98007393"/>    
    <!-- Importing everthing needed. Hang on to your ontological tuque. -->
    <owl:imports rdf:resource="http://purl.org/dc/terms/"/>
    <owl:imports rdf:resource="http://purl.org/ontology/bibo/"/>
    <owl:imports rdf:resource="http://www.w3.org/2004/02/skos/core#"/>
    <owl:imports rdf:resource="http://id.loc.gov/vocabulary/relators/"/>
    <owl:imports rdf:resource="http://xmlns.com/foaf/0.1/"/>
    <owl:imports rdf:resource="http://www.w3.org/ns/prov#"/>
    <owl:imports rdf:resource="http://sparql.cwrc.ca/ontologies/genre#"/>
  </owl:Ontology>
  
  <dcat:Distribution rdf:about="#datasetdefinition-sparql">
   <dcat:accessURL rdf:resource="http://canlink.library.ualberta.ca/sparql"/>
   <rdfs:isDefinedBy rdf:resource="http://canlink.library.ualberta.ca/ontologies/canlink"/>
  </dcat:Distribution>


  <rdf:Description rdf:about="#datasetdefinition">
    <rdfs:isDefinedBy rdf:resource="http://canlink.library.ualberta.ca/ontologies/canlink"/>
    <dcterms:modified rdf:datatype="http://www.w3.org/2001/XMLSchema#Date">DATE_TODAY</dcterms:modified>
    <rdf:type rdf:resource="http://rdfs.org/ns/void#Dataset"/>
    <rdf:type rdf:resource="http://www.w3.org/ns/dcat#Dataset"/>
    <dcat:distribution rdf:resource="#datasetdefinition-sparql"/>
    <void:uriRegexPattern>http://canlink.library.ualberta.ca/.+</void:uriRegexPattern>
    <foaf:homepage rdf:resource="https://connect.library.utoronto.ca/display/U5LD/Canadian+Linked+Data+Initiative+Home"/>
    <void:exampleResource rdf:resource="http://canlink.library.ualberta.ca/"/>
    <void:sparqlEndpoint rdf:resource="http://canlink.library.ualberta.ca/sparql" />
    <void:dataDump rdf:resource="http://canlink.library.ualberta.ca/downloads/"/>
    <void:feature rdf:resource="http://www.w3.org/ns/formats/RDF_XML"/>
    <void:feature rdf:resource="http://www.w3.org/ns/formats/N-Triples"/>
    <void:feature rdf:resource="http://www.w3.org/ns/formats/Turtle"/>
    <void:feature rdf:resource="http://www.w3.org/ns/formats/SPARQL_Results_XML"/>
    <void:feature rdf:resource="http://www.w3.org/ns/formats/SPARQL_Results_JSON"/>
    <void:feature rdf:resource="http://www.w3.org/ns/formats/SPARQL_Results_TSV"/>
    <void:vocabulary rdf:resource="http://purl.org/vocab/vann/"/>
    <void:vocabulary rdf:resource="http://xmlns.com/foaf/spec/"/>
    <void:vocabulary rdf:resource="http://dbpedia.org/resource/"/>
    <void:vocabulary rdf:resource="http://www.w3.org/2006/time#"/>  
    <void:vocabulary rdf:resource="http://creativecommons.org/ns#"/>
    <void:vocabulary rdf:resource="http://www.w3.org/2004/02/skos/core#"/>
    <void:vocabulary rdf:resource="http://www.w3.org/ns/prov#"/>
    <void:vocabulary rdf:resource="http://www.w3.org/2003/06/sw-vocab-status/ns#"/>
    <void:vocabulary rdf:resource="http://www.w3.org/2003/11/swrl#"/>
    <void:vocabulary rdf:resource="http://usefulinc.com/ns/doap#"/>
    <void:vocabulary rdf:resource="http://purl.org/dc/terms/"/>
    <void:vocabulary rdf:resource="http://www.w3.org/TR/void/"/>
    <void:vocabulary rdf:resource="http://www.w3.org/2003/11/swrlb#"/>
    <void:triples>TOTAL_TRIPLES_CLDI</void:triples>
    <void:entities>TOTAL_ENTITIES_CLDI</void:entities>
    <dcterms:title xml:lang="en">The CanLink Ontology</dcterms:title>
    <rdfs:label xml:lang="en">The CanLink Ontology</rdfs:label>
    <foaf:name xml:lang="en">The CanLink Ontology</foaf:name>
    <dcterms:title xml:lang="fr">L'Ontologie CanLien</dcterms:title>
    <rdfs:label xml:lang="fr">L'Ontologie CanLien</rdfs:label>
    <foaf:name xml:lang="fr">L'Ontologie CanLien</foaf:name>
    <dcterms:description xml:lang="en">The CanLink ontology ties together several vocabularies to represent a Canadian thesis collection.</dcterms:description>
    <skos:definition xml:lang="en">The CanLink ontology ties together several vocabularies to represent a Canadian thesis collection.</skos:definition>
    <rdfs:comment xml:lang="en">The CanLink ontology ties together several vocabularies to represent a Canadian thesis collection.</rdfs:comment>
    <dcterms:description xml:lang="fr">L'ontologie CanLien lie plusieurs vocabulaires pour représenter une collection de thèses canadiennes.</dcterms:description>
    <skos:definition xml:lang="fr">L'ontologie CanLien lie plusieurs vocabulaires pour représenter une collection de thèses canadiennes.</skos:definition>
    <rdfs:comment xml:lang="fr">L'ontologie CanLien lie plusieurs vocabulaires pour représenter une collection de thèses canadiennes.</rdfs:comment>
    <dc:date rdf:datatype="http://www.w3.org/2001/XMLSchema#date">DATE_TODAY</dc:date>
    <dc:rights rdf:resource="http://creativecommons.org/licenses/by-nc/4.0/"/> 
    <dc:creator rdf:resource="#RobWarren"/>
    <dc:creator rdf:resource="#SharonFarnel"/>
    <dc:creator rdf:resource="#MaharshPatel"/>
    <dc:publisher>
      <foaf:Organization rdf:about="#CLDI">
        <foaf:name xml:lang="fr">L'initiative Canadiennes des Données Liées</foaf:name>
        <foaf:name xml:lang="en">Canadian Linked Data Initiative</foaf:name>
        <foaf:member rdf:resource="#MaharshPatel"/>
        <foaf:member rdf:resource="#RobertWarren"/>
        <foaf:member rdf:resource="#SharonFarnel"/>
        <foaf:homepage rdf:resource="https://connect.library.utoronto.ca/display/U5LD/Canadian+Linked+Data+Initiative+Home"/>
        <foaf:account>
         <foaf:OnlineAccount rdf:about="#CLDItwitterHandle">
          <rdf:type rdf:resource="http://xmlns.com/foaf/0.1/OnlineChatAccount"/>
          <foaf:accountServiceHomepage rdf:resource="http://www.twitter.com/"/>
        <foaf:accountName>canlink207</foaf:accountName>
       </foaf:OnlineAccount>
      </foaf:account>
      </foaf:Organization>
    </dc:publisher>
    <!-- Electronic dissertations  -->
    <dc:subject rdf:resource="http://id.loc.gov/authorities/subjects/sh98007393"/>
  </rdf:Description>

  <!-- Glue to assign University membership -->
  <rdf:Description rdf:about="http://dbpedia.org/resource/University_of_Alberta">
   <foaf:member rdf:resource="#MaharshPatel"/>
   <foaf:member rdf:resource="#SharonFarnel"/>
  </rdf:Description>

  <!-- Ontology starts here -->  
  
  <owl:DatatypeProperty rdf:about="#pid">
   <skos:definition xml:lang="fr">Le numéros de procédé Unix</skos:definition>
   <skos:definition xml:lang="en">Unix process number for a job</skos:definition>    
   <rdfs:comment xml:lang="en">Used by CanLink to track transformation processes on the server.</rdfs:comment>
   <rdfs:comment xml:lang="fr">Utilisé par CanLink pour suivre les processus de transformation sur le serveur.</rdfs:comment>
   <void:inDataset rdf:resource="#datasetdefinition"/>
   <rdfs:isDefinedBy rdf:resource="http://canlink.library.ualberta.ca/ontologies/canlink"/>
  </owl:DatatypeProperty>

<rdf:Description rdf:about="http://sparql.cwrc.ca/ontologies/genre#hasGenre">
 <rdfs:domain rdf:resource="http://purl.org/ontology/bibo/thesis"/>
 <rdfs:range rdf:resource="http://sparql.cwrc.ca/ontologies/genre#Genre"/>
 <void:inDataset rdf:resource="#datasetdefinition"/>
 <rdfs:isDefinedBy rdf:resource="http://canlink.library.ualberta.ca/ontologies/canlink"/>
 <rdfs:comment xml:lang="en">Thesis are linked to the genre ontology, instances are provided in the datasets.</rdfs:comment>
 <rdfs:comment xml:lang="fr">Les thèses ont un genre; l'instance est déclarée dans l'information.</rdfs:comment> 
</rdf:Description>

<rdf:Description rdf:about="http://purl.org/dc/terms/language">
 <rdf:type rdf:resource="http://www.w3.org/2002/07/owl#ObjectProperty"/>
 <rdfs:domain rdf:resource="http://purl.org/ontology/bibo/thesis"/>
 <rdfs:range rdf:resource="http://id.loc.gov/vocabulary/languages"/>
 <void:inDataset rdf:resource="#datasetdefinition"/>
 <rdfs:isDefinedBy rdf:resource="http://canlink.library.ualberta.ca/ontologies/canlink"/>
 <rdfs:comment xml:lang="en">Most thesis are unilingual and their language is listed in the record.</rdfs:comment>
 <rdfs:comment xml:lang="fr">Les thèses sont unilingue et le language viens du record MARC.</rdfs:comment>
</rdf:Description>

<rdf:Description rdf:about="http://schema.org/encodesCreativeWork">
 <rdf:type rdf:resource="http://www.w3.org/2002/07/owl#ObjectProperty"/>
 <rdfs:domain rdf:resource="http://purl.org/ontology/bibo/thesis"/>
 <rdfs:range rdf:resource="http://purl.org/vocab/frbr/core#Manifestation"/>
 <void:inDataset rdf:resource="#datasetdefinition"/>
 <rdfs:isDefinedBy rdf:resource="http://canlink.library.ualberta.ca/ontologies/canlink"/>
 <rdfs:comment xml:lang="en">Link thesis expression to thesis manifestation.</rdfs:comment>
 <rdfs:comment xml:lang="fr">Lié les expressions de thèses à leurs manifestations.</rdfs:comment>
</rdf:Description>

<rdf:Description rdf:about="http://schema.org/contentURL">
 <rdf:type rdf:resource="http://www.w3.org/2002/07/owl#DatatypeProperty"/>
 <rdfs:domain rdf:resource="http://purl.org/vocab/frbr/core#Manifestation"/>
 <void:inDataset rdf:resource="#datasetdefinition"/>
 <rdfs:isDefinedBy rdf:resource="http://canlink.library.ualberta.ca/ontologies/canlink"/>
 <rdfs:comment xml:lang="en">Link thesis manifestation to it's pdf file.</rdfs:comment>
 <rdfs:comment xml:lang="fr">Lié la manifestation à son fichier pdf.</rdfs:comment>
</rdf:Description>

<rdf:Description rdf:about="http://www.w3.org/ns/prov#wasGeneratedBy">
 <rdfs:domain rdf:resource="http://purl.org/ontology/bibo/thesis"/>
 <rdfs:domain rdf:resource="http://xmlns.com/foaf/0.1/Person"/>
 <rdfs:range rdf:resource="http://www.w3.org/ns/prov#marclodconverter"/>
 <void:inDataset rdf:resource="#datasetdefinition"/>
 <rdfs:isDefinedBy rdf:resource="http://canlink.library.ualberta.ca/ontologies/canlink"/>
 <rdfs:comment xml:lang="en">Documents each run of the converter.</rdfs:comment>
 <rdfs:comment xml:lang="fr">Documente chanque instance du processus de conversion.</rdfs:comment>
</rdf:Description>


<rdf:Description rdf:about="http://purl.org/dc/terms/issued">
 <rdf:type rdf:resource="http://www.w3.org/2002/07/owl#DatatypeProperty"/>
 <rdfs:domain rdf:resource="http://purl.org/ontology/bibo/thesis"/>
 <void:inDataset rdf:resource="#datasetdefinition"/>
 <rdfs:isDefinedBy rdf:resource="http://canlink.library.ualberta.ca/ontologies/canlink"/>
 <rdfs:comment xml:lang="en">Deposit date.</rdfs:comment>
 <rdfs:comment xml:lang="fr">Date de dépot.</rdfs:comment>
</rdf:Description>

<rdf:Description rdf:about="http://purl.org/dc/terms/title">
 <rdf:type rdf:resource="http://www.w3.org/2002/07/owl#DatatypeProperty"/>
 <rdfs:domain rdf:resource="http://purl.org/ontology/bibo/thesis"/>
 <void:inDataset rdf:resource="#datasetdefinition"/>
 <rdfs:isDefinedBy rdf:resource="http://canlink.library.ualberta.ca/ontologies/canlink"/>
 <rdfs:comment xml:lang="en">Title is not enforced by BIBO, but we do.</rdfs:comment>
 <rdfs:comment xml:lang="fr">L'ontogie BIBO ne force pas un titre, donc on le fait ici.</rdfs:comment>
</rdf:Description>

<rdf:Description rdf:about="http://purl.org/dc/terms/publisher">
 <rdf:type rdf:resource="http://www.w3.org/2002/07/owl#ObjectProperty"/>
 <rdfs:domain rdf:resource="http://purl.org/ontology/bibo/thesis"/>
 <rdfs:range rdf:resource="http://www.w3.org/2004/02/skos/core#Concept"/>
 <void:inDataset rdf:resource="#datasetdefinition"/>
 <rdfs:isDefinedBy rdf:resource="http://canlink.library.ualberta.ca/ontologies/canlink"/>
 <rdfs:comment xml:lang="en">CLDI will state publisher using both LOC and DCTERMS.</rdfs:comment>
 <rdfs:comment xml:lang="fr">ICDL émet le triplet LOC ainsi que le DC pour le publicateur.</rdfs:comment>
</rdf:Description>

<rdf:Description rdf:about="http://id.loc.gov/vocabulary/relators/pbl">
 <rdf:type rdf:resource="http://www.w3.org/2002/07/owl#ObjectProperty"/>
 <rdfs:domain rdf:resource="http://purl.org/ontology/bibo/thesis"/>
 <rdfs:range rdf:resource="http://www.w3.org/2004/02/skos/core#Concept"/>
 <void:inDataset rdf:resource="#datasetdefinition"/>
 <rdfs:isDefinedBy rdf:resource="http://canlink.library.ualberta.ca/ontologies/canlink"/>
 <rdfs:comment xml:lang="en">CLDI will state publisher using both LOC and DCTERMS.</rdfs:comment>
 <rdfs:comment xml:lang="fr">ICDL émet le triplet LOC ainsi que le DC pour le publicateur.</rdfs:comment>
</rdf:Description>

<rdf:Description rdf:about="http://id.loc.gov/vocabulary/relators/ths">
 <rdf:type rdf:resource="http://www.w3.org/2002/07/owl#ObjectProperty"/>
 <rdfs:range rdf:resource="http://xmlns.com/foaf/0.1/Person"/>
 <void:inDataset rdf:resource="#datasetdefinition"/>
 <rdfs:isDefinedBy rdf:resource="http://canlink.library.ualberta.ca/ontologies/canlink"/>
 <rdfs:comment xml:lang="en">Not all thesis records list their advisors, but when they do, it makes use of FOAF to represent advisor.</rdfs:comment>
 <rdfs:comment xml:lang="fr">Certaine des thèses enregistre l'adviseur et le FOAF est utilisé pour cet information. </rdfs:comment>
</rdf:Description>


<rdf:Description rdf:about="http://purl.org/dc/terms/creator">
 <rdf:type rdf:resource="http://www.w3.org/2002/07/owl#ObjectProperty"/>
 <rdfs:domain rdf:resource="http://purl.org/ontology/bibo/thesis"/>
 <rdfs:range rdf:resource="http://xmlns.com/foaf/0.1/Person"/>
 <void:inDataset rdf:resource="#datasetdefinition"/>
 <rdfs:isDefinedBy rdf:resource="http://canlink.library.ualberta.ca/ontologies/canlink"/>
 <rdfs:comment xml:lang="en">CLDI will state author using both LOC and DCTERMS.</rdfs:comment>
 <rdfs:comment xml:lang="fr">ICDL émet le triplet LOC ainsi que le DC pour l'auteur.</rdfs:comment>
</rdf:Description>

<rdf:Description rdf:about="http://id.loc.gov/vocabulary/relators/aut">
 <rdf:type rdf:resource="http://www.w3.org/2002/07/owl#ObjectProperty"/>
 <rdfs:domain rdf:resource="http://purl.org/ontology/bibo/thesis"/>
 <rdfs:range rdf:resource="http://xmlns.com/foaf/0.1/Person"/>
 <void:inDataset rdf:resource="#datasetdefinition"/>
 <rdfs:isDefinedBy rdf:resource="http://canlink.library.ualberta.ca/ontologies/canlink"/>
 <rdfs:comment xml:lang="en">CLDI will state author using both LOC and DCTERMS.</rdfs:comment>
 <rdfs:comment xml:lang="fr">ICDL émet le triplet LOC ainsi que le DC pour l'auteur.</rdfs:comment>
</rdf:Description>

<!-- This should work for BNF also -->
<rdf:Description rdf:about="http://purl.org/dc/terms/subject">
 <rdf:type rdf:resource="http://www.w3.org/2002/07/owl#ObjectProperty"/>
 <rdfs:domain rdf:resource="http://purl.org/ontology/bibo/thesis"/>
 <rdfs:range rdf:resource="http://id.loc.gov/authorities/subjects"/>
 <rdfs:range rdf:resource="http://www.w3.org/2004/02/skos/core#Concept"/>
 <void:inDataset rdf:resource="#datasetdefinition"/>
 <rdfs:isDefinedBy rdf:resource="http://canlink.library.ualberta.ca/ontologies/canlink"/>
 <rdfs:comment xml:lang="en">CLDI makes use of either LCHS or basic SKOS for subjects.</rdfs:comment>
 <rdfs:comment xml:lang="fr">L'ICDL utilise soit les sujets LCHS ou un concept SKOS.</rdfs:comment>
</rdf:Description>

<prov:Activity rdf:about="#marclodconverter">
 <rdf:type rdf:resource="http://usefulinc.com/ns/doap#Project"/>
 <rdfs:label xml:lang="en">The CanLink MARC/LOD Converter Software</rdfs:label> 
 <rdfs:label xml:lang="fr">Le convertisseur CanaLien MARC/LOD</rdfs:label> 
 <doap:name xml:lang="en">The CanLink MARC/LOD Converter Software</doap:name> 
 <doap:name xml:lang="fr">Le convertisseur CanaLien MARC/LOD</doap:name> 
 <doap:homepage rdf:resource="http://canlink.library.ualberta.ca/"/>
 <doap:category rdf:resource="http://id.loc.gov/authorities/subjects/sh98007393"/>
 <doap:license rdf:resource="http://creativecommons.org/licenses/by-nc/4.0/"/>
 <doap:service-endpoint rdf:resource="http://canlink.library.ualberta.ca/"/>
 <doap:language rdf:resource="http://id.loc.gov/vocabulary/languages/eng"/>
 <doap:language rdf:resource="http://id.loc.gov/vocabulary/languages/fre"/>
 <doap:programming-language rdf:resource="https://en.wikipedia.org/wiki/Python_(programming_language)"/> 
 <doap:developer rdf:resource="#SharonFarnel"/>
 <doap:developer rdf:resource="#RobWarren"/>
 <doap:developer rdf:resource="#MaharshPatel"/>
 <dc:publisher rdf:resource="#CLDI"/>
 <doap:shortdesc xml:lang="en">Converts MARC format thesis records into Linked Open Data records.</doap:shortdesc>
 <doap:shortdesc xml:lang="fr">Convertie les records MARC en données liées.</doap:shortdesc>
 <doap:repository>
  <doap:GitRepository rdf:about="#canlinkrepo">
   <doap:location rdf:resource="https://github.com/cldi/CanLink.git"/>
   <doap:browse rdf:resource="https://github.com/cldi/CanLink/"/>
  </doap:GitRepository>
 </doap:repository>
 <void:inDataset rdf:resource="#datasetdefinition"/>
 <rdfs:isDefinedBy rdf:resource="http://canlink.library.ualberta.ca/ontologies/canlink"/>
</prov:Activity>

</rdf:RDF>
