<?xml version="1.0"?>
<rdf:RDF xml:base="http://canlink.library.ualberta.ca/ontologies/canlink#" 
  xmlns="http://canlink.library.ualberta.ca/ontologies/canlink#" 
  xmlns:as="http://www.w3.org/ns/activitystreams#" 
  xmlns:bio="http://purl.org/vocab/bio/0.1/" 
  xmlns:cc="http://creativecommons.org/ns#" 
  xmlns:cwrc="http://canlink.library.ualberta.ca/ontologies/canlink#" 
  xmlns:dbpedia="http://dbpedia.org/resource/" 
  xmlns:dcterms="http://purl.org/dc/terms/" 
  xmlns:doap="http://usefulinc.com/ns/doap#" 
  xmlns:bibo="http://purl.org/ontology/bibo/"
  xmlns:foaf="http://xmlns.com/foaf/0.1/" 
  xmlns:loc="http://id.loc.gov/vocabulary/relators/" 
  xmlns:locl ="http://id.loc.gov/vocabulary/languages/"
  xmlns:nif="http://persistence.uni-leipzig.org/nlp2rdf/ontologies/nif-core#" 
  xmlns:oa="http://www.w3.org/ns/oa#" 
  xmlns:owl="http://www.w3.org/2002/07/owl#" 
  xmlns:prov="http://www.w3.org/ns/prov#" 
  xmlns:rdf="http://www.w3.org/1999/02/22-rdf-syntax-ns#" 
  xmlns:rdfs="http://www.w3.org/2000/01/rdf-schema#" 
  xmlns:rel="http://purl.org/vocab/relationship/" 
  xmlns:skos="http://www.w3.org/2004/02/skos/core#" 
  xmlns:skosxl="http://www.w3.org/2008/05/skos-xl#" 
  xmlns:time="http://www.w3.org/2006/time#" 
  xmlns:vann="http://purl.org/vocab/vann/" 
  xmlns:voaf="http://purl.org/vocommons/voaf#" 
  xmlns:void="http://rdfs.org/ns/void#" 
  xmlns:vs="http://www.w3.org/2003/06/sw-vocab-status/ns#" 
  xmlns:xsd="http://www.w3.org/2001/XMLSchema#">

  <owl:Ontology rdf:about="">
    <rdf:type rdf:resource="http://purl.org/vocommons/voaf#Vocabulary"/>
    <dcterms:title xml:lang="en">The CanLink Ontology</dcterms:title>
    <rdfs:label xml:lang="en">The CanLink Ontology</rdfs:label>
    <foaf:name xml:lang="en">The CanLink Ontology</foaf:name>
    <dcterms:title xml:lang="fr">L'Ontologie CanLink</dcterms:title>
    <rdfs:label xml:lang="fr">L'Ontologie CanLink</rdfs:label>
    <foaf:name xml:lang="fr">L'Ontologie CanLink</foaf:name>
    <dcterms:description xml:lang="en">The CanLink ontology ties together several vocabularies to represent a Canadian thesis collection.</dcterms:description>
    <skos:definition xml:lang="en">The CanLink ontology ties together several vocabularies to represent a Canadian thesis collection.</skos:definition>
    <rdfs:comment xml:lang="en">The CanLink ontology ties together several vocabularies to represent a Canadian thesis collection.</rdfs:comment>
    <dcterms:description xml:lang="fr">L'ontologie CanLink lie plusieurs vocabulaires pour représenter une collection de thèses canadiennes.</dcterms:description>
    <skos:definition xml:lang="fr">L'ontologie CanLink lie plusieurs vocabulaires pour représenter une collection de thèses canadiennes.</skos:definition>
    <rdfs:comment xml:lang="fr">L'ontologie CanLink lie plusieurs vocabulaires pour représenter une collection de thèses canadiennes.</rdfs:comment>
    <owl:versionInfo>1.0</owl:versionInfo>
    <dcterms:date rdf:datatype="http://www.w3.org/2001/XMLSchema#date">DATE_TODAY</dcterms:date>
    <dcterms:rights rdf:resource="http://creativecommons.org/licenses/by-nc/4.0/"/>
    <vs:term_status xml:lang="en">Testing</vs:term_status>
    <dcterms:creator>
      <foaf:Person rdf:about="#RobWarren">
        <foaf:name>Robert Warren</foaf:name>
        <owl:sameAs rdf:resource="http://rdf.muninn-project.org/ww1/2011/11/11/Person/Warren"/>
      </foaf:Person>
    </dcterms:creator>
    <dcterms:creator>
      <foaf:Person rdf:about="#SharonFarnel">
        <foaf:name>Sharon Farnel</foaf:name>
      </foaf:Person>
    </dcterms:creator>
    <dcterms:creator>
      <foaf:Person rdf:about="#MaharshPatel">
        <foaf:name>Maharsh Patel</foaf:name>
      </foaf:Person>
    </dcterms:creator>
    <dcterms:publisher rdf:resource="http://canlink.library.ualberta.ca/.well-know/void#CLDI"/>
    <void:inDataset rdf:resource="http://canlink.library.ualberta.ca/.well-know/void#datasetdefinition"/>
    <rdfs:isDefinedBy rdf:resource="http://canlink.library.ualberta.ca/ontologies/canlink"/>
    <!-- Electronic dissertations  -->
    <dcterms:subject rdf:resource="http://id.loc.gov/authorities/subjects/sh98007393"/>
    <!-- Dissertations, Academic -->
    <dcterms:subject rdf:resource="http://id.loc.gov/authorities/subjects/sh98007393"/>
  </owl:Ontology>
  
  <owl:DatatypeProperty rdf:about="#pid">
   <skos:definition xml:lang="fr">Le numéros de procédé Unix</skos:definition>
   <skos:definition xml:lang="en">Unix process number for a job</skos:definition>    
   <rdfs:comment xml:lang="en">Used by CanLink to track transformation processes on the server.</rdfs:comment>
   <rdfs:comment xml:lang="fr">Utilisé par CanLink pour suivre les processus de transformation sur le serveur.</rdfs:comment>
   <void:inDataset rdf:resource="http://canlink.library.ualberta.ca/.well-know/void#datasetdefinition"/>
   <rdfs:isDefinedBy rdf:resource="http://canlink.library.ualberta.ca/ontologies/canlink"/>
  </owl:DatatypeProperty>

<rdf:Description rdf:about="http://purl.org/dc/terms/language">
 <rdfs:domain rdf:resource="http://purl.org/ontology/bibo/thesis"/>
 <rdfs:range rdf:resource="http://id.loc.gov/vocabulary/languages"/>
 <void:inDataset rdf:resource="http://canlink.library.ualberta.ca/.well-know/void#datasetdefinition"/>
 <rdfs:isDefinedBy rdf:resource="http://canlink.library.ualberta.ca/ontologies/canlink"/>
 <rdfs:comment xml:lang="en">Most thesis are unilingual and their language is listed in the record.</rdfs:comment>
 <rdfs:comment xml:lang="fr">Les thèses sont unilingue et le language viens du record MARC.</rdfs:comment>
</rdf:Description>

<rdf:Description rdf:about="http://purl.org/dc/terms/issued">
 <rdfs:domain rdf:resource="http://purl.org/ontology/bibo/thesis"/>
 <void:inDataset rdf:resource="http://canlink.library.ualberta.ca/.well-know/void#datasetdefinition"/>
 <rdfs:isDefinedBy rdf:resource="http://canlink.library.ualberta.ca/ontologies/canlink"/>
 <rdfs:comment xml:lang="en">Deposit date.</rdfs:comment>
 <rdfs:comment xml:lang="fr">Date de dépot.</rdfs:comment>
</rdf:Description>

<rdf:Description rdf:about="http://purl.org/dc/terms/title">
 <rdfs:domain rdf:resource="http://purl.org/ontology/bibo/thesis"/>
 <void:inDataset rdf:resource="http://canlink.library.ualberta.ca/.well-know/void#datasetdefinition"/>
 <rdfs:isDefinedBy rdf:resource="http://canlink.library.ualberta.ca/ontologies/canlink"/>
 <rdfs:comment xml:lang="en">Title is not enforced by BIBO, but we do.</rdfs:comment>
 <rdfs:comment xml:lang="fr">L'ontogie BIBO ne force pas un titre, donc on le fait ici.</rdfs:comment>
</rdf:Description>

<rdf:Description rdf:about="http://purl.org/dc/terms/publisher">
 <rdfs:domain rdf:resource="http://purl.org/ontology/bibo/thesis"/>
 <rdfs:range rdf:resource="http://www.w3.org/2004/02/skos/core#Concept"/>
 <void:inDataset rdf:resource="http://canlink.library.ualberta.ca/.well-know/void#datasetdefinition"/>
 <rdfs:isDefinedBy rdf:resource="http://canlink.library.ualberta.ca/ontologies/canlink"/>
 <rdfs:comment xml:lang="en">CLDI will state publisher using both LOC and DCTERMS.</rdfs:comment>
 <rdfs:comment xml:lang="fr">ICDL émet le triplet LOC ainsi que le DC pour le publicateur.</rdfs:comment>
</rdf:Description>

<rdf:Description rdf:about="http://id.loc.gov/vocabulary/relators/pbl">
 <rdfs:domain rdf:resource="http://purl.org/ontology/bibo/thesis"/>
 <rdfs:range rdf:resource="http://www.w3.org/2004/02/skos/core#Concept"/>
 <void:inDataset rdf:resource="http://canlink.library.ualberta.ca/.well-know/void#datasetdefinition"/>
 <rdfs:isDefinedBy rdf:resource="http://canlink.library.ualberta.ca/ontologies/canlink"/>
 <rdfs:comment xml:lang="en">CLDI will state publisher using both LOC and DCTERMS.</rdfs:comment>
 <rdfs:comment xml:lang="fr">ICDL émet le triplet LOC ainsi que le DC pour le publicateur.</rdfs:comment>
</rdf:Description>

<rdf:Description rdf:about="http://id.loc.gov/vocabulary/relators/ths">
 <rdfs:range rdf:resource="http://xmlns.com/foaf/0.1/Person"/>
 <void:inDataset rdf:resource="http://canlink.library.ualberta.ca/.well-know/void#datasetdefinition"/>
 <rdfs:isDefinedBy rdf:resource="http://canlink.library.ualberta.ca/ontologies/canlink"/>
 <rdfs:comment xml:lang="en">Not all thesis records list their advisors, but when they do, it makes use of FOAF to represent advisor.</rdfs:comment>
 <rdfs:comment xml:lang="fr">Certaine des thèses enregistre l'adviseur et le FOAF est utilisé pour cet information. </rdfs:comment>
</rdf:Description>


<rdf:Description rdf:about="http://purl.org/dc/terms/creator">
 <rdfs:domain rdf:resource="http://purl.org/ontology/bibo/thesis"/>
 <rdfs:range rdf:resource="http://xmlns.com/foaf/0.1/Person"/>
 <void:inDataset rdf:resource="http://canlink.library.ualberta.ca/.well-know/void#datasetdefinition"/>
 <rdfs:isDefinedBy rdf:resource="http://canlink.library.ualberta.ca/ontologies/canlink"/>
 <rdfs:comment xml:lang="en">CLDI will state author using both LOC and DCTERMS.</rdfs:comment>
 <rdfs:comment xml:lang="fr">ICDL émet le triplet LOC ainsi que le DC pour l'auteur.</rdfs:comment>
</rdf:Description>

<rdf:Description rdf:about="http://id.loc.gov/vocabulary/relators/aut">
 <rdfs:domain rdf:resource="http://purl.org/ontology/bibo/thesis"/>
 <rdfs:range rdf:resource="http://xmlns.com/foaf/0.1/Person"/>
 <void:inDataset rdf:resource="http://canlink.library.ualberta.ca/.well-know/void#datasetdefinition"/>
 <rdfs:isDefinedBy rdf:resource="http://canlink.library.ualberta.ca/ontologies/canlink"/>
 <rdfs:comment xml:lang="en">CLDI will state author using both LOC and DCTERMS.</rdfs:comment>
 <rdfs:comment xml:lang="fr">ICDL émet le triplet LOC ainsi que le DC pour l'auteur.</rdfs:comment>
</rdf:Description>

<rdf:Description rdf:about="http://purl.org/dc/terms/subject">
 <rdfs:domain rdf:resource="http://purl.org/ontology/bibo/thesis"/>
 <rdfs:range rdf:resource="http://id.loc.gov/authorities/subjects"/>
 <rdfs:range rdf:resource="http://www.w3.org/2004/02/skos/core#Concept"/>
 <void:inDataset rdf:resource="http://canlink.library.ualberta.ca/.well-know/void#datasetdefinition"/>
 <rdfs:isDefinedBy rdf:resource="http://canlink.library.ualberta.ca/ontologies/canlink"/>
 <rdfs:comment xml:lang="en">CLDI makes use of either LCHS or basic SKOS for subjects.</rdfs:comment>
 <rdfs:comment xml:lang="fr">L'ICDL utilise soit les sujets LCHS ou un concept SKOS.</rdfs:comment>
</rdf:Description>

<prov:Activity rdf:about="#marclodconverter">
 <rdf:type rdf:resource="http://usefulinc.com/ns/doap#Project"/>
 <rdfs:label xml:lang="en">The CanLink MARC/LOD Converter Software</rdfs:label> 
 <rdfs:label xml:lang="fr">Le convertisseur CanaLien MARC/LOD</rdfs:label> 
 <doap:name xml:lang="en">The CanLink MARC/LOD Converter Software</doap:name> 
 <doap:name xml:lang="fr">Le convertisseur CanaLien MARC/LOD</doap:name> 
 <doap:homepage rdf:resource="http://canlink.library.ualberta.ca/"/>
 <doap:category rdf:resource="http://id.loc.gov/authorities/subjects/sh98007393"/>
 <doap:license rdf:resource="http://creativecommons.org/licenses/by-nc/4.0/"/>
 <doap:service-endpoint rdf:resource="http://canlink.library.ualberta.ca/"/>
 <doap:language rdf:resource="http://id.loc.gov/vocabulary/languages/eng"/>
 <doap:language rdf:resource="http://id.loc.gov/vocabulary/languages/fre"/>
 <doap:programming-language rdf:resource="https://en.wikipedia.org/wiki/Python_(programming_language)"/> 
 <doap:developer rdf:resource="#SharonFarnel"/>
 <doap:developer rdf:resource="#RobWarren"/>
 <doap:developer rdf:resource="#MaharshPatel"/>
 <doap:shortdesc xml:lang="en">Converts MARC format thesis records into Linked Open Data records.</doap:shortdesc>
 <doap:shortdesc xml:lang="fr">Convertie les records MARC en données liées.</doap:shortdesc>
 <doap:repository>
  <doap:GitRepository rdf:about="#canlinkrepo">
   <doap:location rdf:resource="https://github.com/cldi/CanLink.git"/>
   <doap:browse rdf:resource="https://github.com/cldi/CanLink/"/>
  </doap:GitRepository>
 </doap:repository>
</prov:Activity>

</rdf:RDF>
